CC/Typed/TypeSubst.lean
@@ -1,0 +1,89 @@
+import Mathlib.Data.Fin.Basic
+import CC.Basic
+import CC.Rename
+import CC.CaptureSet
+import CC.Type
+import CC.Type.TypeSubst
+import CC.Term.TypeSubst
+import CC.Context
+import CC.TypeMap
+import CC.Subst
+import CC.Typed
+import CC.Typed.Basic
+import CC.Subtype
+import CC.Narrowing
+import CC.Subtype.TypeSubst
+
+namespace CC
+
+def Typed.tsubst {Δ : Ctx n m2}
+  (h : Typed Γ t C T)
+  (σ : VarTypeMap Γ Δ g)
+  (δ : TVarSubst Γ Δ g) :
+  Typed Δ (t.tsubst g) C (T.tsubst g) := by
+  induction h generalizing m2
+  case var hb =>
+    simp [Term.tsubst, CType.tsubst]
+    have hb' := σ hb
+    simp [CType.tsubst] at hb'
+    constructor; trivial
+  case sub ih =>
+    apply Typed.sub
+    apply ih <;> trivial
+    apply Subtype.tsubst <;> trivial
+  case abs ih =>
+    simp [Term.tsubst]
+    apply Typed.abs
+    apply ih
+    apply VarTypeMap.ext_var; trivial
+    apply TVarSubst.ext_var; trivial
+    trivial
+  case tabs ih =>
+    simp [Term.tsubst]
+    apply Typed.tabs
+    apply ih
+    apply VarTypeMap.ext_tvar; trivial
+    apply TVarSubst.ext_tvar; trivial
+  case app ih1 ih2 =>
+    simp [Term.tsubst]
+    rw [CType.tsubst_open_var_comm]
+    simp [Term.tsubst] at ih1 ih2
+    apply Typed.app
+    apply ih1 <;> trivial
+    apply ih2 <;> trivial
+    trivial
+  case tapp ih =>
+    simp [Term.tsubst]
+    rw [CType.tsubst_open_tvar_comm]
+    simp [Term.tsubst] at ih
+    apply Typed.tapp
+    apply ih <;> trivial
+  case box ih =>
+    simp [Term.tsubst] at *
+    apply Typed.box
+    apply ih <;> trivial
+  case unbox ih =>
+    simp [Term.tsubst] at *
+    apply Typed.unbox
+    apply ih <;> trivial
+  case letval1 ih1 ih2 =>
+    simp [Term.tsubst] at *
+    apply Typed.letval1
+    apply ih1 <;> trivial
+    apply ih2 <;> try trivial
+    apply VarTypeMap.ext_var; trivial
+    apply TVarSubst.ext_var; trivial
+    subst_vars
+    simp [CType.tsubst_weaken_var_comm]
+    trivial
+  case letval2 ih1 ih2 =>
+    simp [Term.tsubst] at *
+    apply Typed.letval2
+    apply ih1 <;> trivial
+    apply Value.tsubst; trivial
+    apply ih2
+    apply VarTypeMap.ext_var; trivial
+    apply TVarSubst.ext_var; trivial
+    subst_vars
+    simp [CType.tsubst_weaken_var_comm]
+    trivial
